Day 2: Restructure & Some Theorems

Gaea/Logic/Basic.lean
@@ -1,9 +1,17 @@
-universes u v w
-
 namespace Gaea
 
-structure Logic :=
-  (prop : Sort u)
-  (proof : prop -> Sort v)
+def Logic.{u,v} (prop : Sort u) 
+  := prop -> Sort v
+
+namespace Logic
+
+def prop.{u,v} {P : Sort u} (L : Logic.{u,v} P) := P
+
+def Proof.{u,v} {P : Sort u} (L : Logic.{u,v} P) := Sort v
+
+def Judgment.{u,v} {P : Sort u} (L : Logic.{u,v} P) (prop : P) 
+  := L prop
+
+end Logic
 
 end Gaea
