Gaea/Peano/Nat.lean
@@ -1,32 +1,17 @@
-import Gaea.Logic
+universes u v
 
 namespace Gaea.Peano
 
-class Nat (L : Logic) :=
-  (form : Sort u)
-  (is_nat : form -> L.prop)
+class Nat (prop : Sort u) (form : Sort v) := 
+  (nat : form -> prop)
 
-class IsNat (prop : Sort u) (form : Sort v) := 
-  (is_nat : form -> prop)
-
-instance (L : Logic) (N : Nat L) : IsNat L.prop N.form :=
-  {is_nat := N.is_nat}
-
-export IsNat (is_nat)
-
-def Shorthand.nat {L : Logic} {N : Nat L} := N.is_nat
-open Shorthand (nat)
+export Nat (nat)
 
 namespace Nat
 
-def pred {L : Logic} (N : Nat L) :=
-  N.form -> L.prop
-
-def Sigma {L : Logic} (N : Nat L) := 
-  _root_.Sigma (fun n : N.form => L.proof (nat n)) 
-
-def sigma {L : Logic} (N : Nat L) : 
-  (n : N.form) -> L.proof (nat n) -> N.Sigma := Sigma.mk
+def prop {P : Sort u} {T : Sort v} (N : Nat P T) := P
+def form {P : Sort u} {T : Sort v} (N : Nat P T) := T
+def pred {P : Sort u} {T : Sort v} (N : Nat P T) := T -> P
 
 end Nat
 
