Gaea/Logic.lean
@@ -1,2 +1,1 @@
 import Gaea.Logic.Basic
-import Gaea.Logic.Syntax
