Gaea/Logic/Rules.lean
@@ -1,0 +1,39 @@
+import Gaea.Logic
+import Gaea.Syntax.Logic
+import Gaea.Logic.Notation
+import Gaea.Syntax.Notation
+
+universes u v
+
+open Gaea.Syntax
+
+namespace Gaea.Logic.Rules
+
+-- Forall
+
+def ForallIntro {P : Sort u} (L : Logic P) (T : Sort v) [LForall P T] := 
+  (f : T -> P) -> ((a : T) -> (L |- f a)) -> (L |- lForall f) 
+
+def ForallElim {P : Sort u} (L : Logic P) (T : Sort v) [LForall P T] := 
+  (f : T -> P) -> (L |- lForall f) -> ((a : T) -> (L |- f a))  
+
+-- If
+
+def IfIntro {P : Sort u} (L : Logic P) [LIf P] := 
+  (p q : P) -> ((L |- p) -> (L |- q)) -> (L |- p -> q) 
+
+def IfElim {P : Sort u} (L : Logic P) [LIf P] := 
+  (p q : P) -> (L |- p -> q) -> ((L |- p) -> (L |- q))  
+
+-- Equality
+
+def EqRefl {P : Sort u} {T : Sort v} (L : Logic P) (C : LEq P T) :=
+  (x : T) -> L |- x = x
+
+def EqSymm {P : Sort u} {T : Sort v} (L : Logic P) (C : LEq P T) :=
+  (x y : T) -> (L |- x = y) -> (L |- y = x)
+
+def EqTrans {P : Sort u} {T : Sort v} (L : Logic P)  (C : LEq P T) :=
+  (x y z : T) -> (L |- x = y) -> (L |- y = z) -> (L |- x = z)
+
+end Gaea.Logic.Rules
