Gaea/Peano/Props.lean
@@ -1,0 +1,69 @@
+import Gaea.Logic
+import Gaea.Peano.Nat
+
+import Gaea.Syntax.Math
+import Gaea.Syntax.Logic
+import Gaea.Syntax.Notation
+import Gaea.Logic.Notation
+
+open Gaea.Logic
+open Gaea.Syntax
+
+namespace Gaea.Peano.Props
+
+universes u v
+
+-- Axiom 1
+def natZero {P : Sort u} (N : Type u) [Nat P N] [Zero N] : P :=
+  nat (0 : N)
+
+-- Axiom 2
+def eqNatRefl {P : Sort u} (N : Sort v) 
+  [LForall P N] [LIf P] [LEq P N] [Nat P N] : P :=
+  forall (x : N) => nat x -> x = x
+
+-- Axiom 3
+def eqNatSymm {P : Sort u} (N : Sort v) 
+  [LForall P N] [LIf P] [LAnd P] [LEq P N] [Nat P N]: P :=
+  forall (x y : N) => nat x /\ nat y -> (x = y -> y = x)
+
+-- Axiom 4
+def eqNatTrans {P : Sort u} (N : Sort v) 
+  [LForall P N] [LIf P] [LAnd P] [LEq P N] [Nat P N] : P :=
+  forall (x y z : N) => nat x /\ nat y /\ nat z -> (x = y /\ y = z -> x = z)
+
+-- Axiom 5
+def natEq {P : Sort u} (L : Logic P) (N : Sort v) 
+  [LForall P N] [LIf P] [LEq P N] [Nat P N] : P :=
+  forall (a b : N) => nat b -> (a = b) -> nat a
+
+-- Axiom 6
+def natSuccNat {P : Sort u} (N : Sort v) 
+  [LForall P N] [LIf P] [Nat P N] [Succ N] : P :=
+  forall (n : N) => nat n -> nat (S n)
+
+-- Axiom 7a
+def succNatSubst {P : Sort u} (N : Sort v) 
+  [LForall P N] [LIf P] [LAnd P] [LEq P N] [Nat P N] [Succ N] : P  :=
+  forall (m n : N) => nat m /\ nat n -> (m = n -> S m = S n)
+
+-- Axiom 7b
+def succNatInj {P : Sort u} (N : Sort v) 
+  [LForall P N] [LIf P] [LAnd P] [LEq P N] [Nat P N] [Succ N] : P  :=
+  forall (m n : N) => nat m /\ nat n -> (S m = S n -> m = n)
+
+-- Axiom 8
+def succNatEqZeroFalse {P : Sort u} (N : Type v) 
+  [LForall P N] [LIf P] [LAnd P] [LEq P N] [Nat P N] [Zero N] [Succ N] [False P] : P  :=
+  forall (m n : N) => nat m /\ nat n -> (S n = 0 -> false)
+
+-- Axiom 9
+def natInduction 
+  {P : Sort u} (N : Type v) [Nat P N] 
+  [LForall P (N -> P)] [LForall P N] [LIf P] [LAnd P] [LEq P N] 
+  [Nat P N] [Zero N] [Succ N] : P := 
+  forall (f : N -> P) => 
+    f 0 -> (forall (n : N) => nat n -> (f n -> f (S n))) ->
+      forall (n : N) => nat n -> f n
+
+end Gaea.Peano.Props
