Gaea/Peano/Rules.lean
@@ -1,0 +1,97 @@
+import Gaea.Logic
+import Gaea.Peano.Nat
+
+import Gaea.Syntax.Math
+import Gaea.Syntax.Logic
+import Gaea.Syntax.Notation
+import Gaea.Logic.Notation
+
+open Gaea.Logic
+open Gaea.Syntax
+
+namespace Gaea.Peano.Rules
+
+universes u v w
+
+-- Natural Axioms
+
+-- Axiom 1
+def NatZero {P : Sort u} (L : Logic P) (N : Type v) [Zero N] [Nat P N] :=
+  L |- nat (0 : N)
+
+-- Axiom 2
+def EqNatRefl {P : Sort u} (L : Logic P) (N : Sort v) [Nat P N] [LEq P N] :=
+  (x : N) -> (L |- nat x) -> (L |- x = x)
+
+-- Axiom 3
+def EqNatSymm {P : Sort u} (L : Logic P) (N : Sort v) [Nat P N] [LEq P N] :=
+  (x y : N) -> (L |- nat x) -> (L |- nat y) ->
+    (L |- x = y) -> (L |- y = x)
+
+-- Axiom 4
+def EqNatTrans {P : Sort u} (L : Logic P) (N : Sort v) [Nat P N] [LEq P N] :=
+  (x y z : N) -> (L |- nat x) -> (L |- nat y) -> (L |- nat z) -> 
+    (L |- x = y) -> (L |- y = z) -> (L |- x = z)
+
+-- Axiom 5
+def NatEq {P : Sort u} (L : Logic P) (N : Sort v) [Nat P N] [LEq P N] :=
+  (a b : N) -> (L |- nat b) -> (L |- a = b) -> (L |- nat a)
+
+-- Axiom 6
+def NatSuccNat {P : Sort u} (L : Logic P) (N : Sort v) [Nat P N] [Succ N]:=
+  (n : N) -> (L |- nat n) -> (L |- nat (S n))
+
+-- Axiom 7a
+def SuccNatSubst 
+  {P : Sort u} (L : Logic P) (N : Sort v) [Nat P N] [LEq P N] [Succ N]  :=
+  (m n : N) -> (L |- nat m) -> (L |- nat n)-> 
+    (L |- m = n) -> (L |- S m = S n)
+
+-- Axiom 7b
+def SuccNatInj 
+  {P : Sort u} (L : Logic P) (N : Sort v) [Nat P N] [LEq P N] [Succ N] :=
+  (m n : N) -> (L |- nat m) -> (L |- nat n) -> 
+    (L |- S m = S n) -> (L |- m = n)
+
+-- Axiom 8
+def SuccNatEqZeroFalse 
+  {P : Sort u} (L : Logic P) (N : Type v) 
+  [Nat P N] [LEq P N] [Succ N] [Zero N] [False P] :=
+  (m n : N) -> (L |- nat m) -> (L |- nat n) -> 
+    (L |- S n = 0) -> (L |- false)
+
+-- Axiom 9
+def NatInduction 
+  {P : Sort u} (L : Logic P) (N : Type v) [Nat P N] [Zero N] [Succ N] := 
+  (f : N -> P) -> (L |- f 0) -> 
+  ((n : N) -> (L |- nat n) -> (L |- f n) -> (L |- f (S n))) ->
+  ((n : N) -> (L |- nat n) -> (L |- f n))
+
+def NatInduction'
+  {P : Sort u} (L : Logic P) (N : Type v) [Nat P N] [Zero N] [Succ N] := 
+  (f : N -> Sort w) -> f 0 ->
+  ((n : N) -> (L |- nat n) -> (f n -> f (S n))) ->
+  ((n : N) -> (L |- nat n) -> f n)
+
+-- Addition Axioms
+
+def AddNatZeroEqNat 
+  {P : Sort u} (L : Logic P) (N : Type v) [LEq P N] [Nat P N] [Zero N] [Add N] :=
+  (a : N) -> (L |- nat a) -> (L |- a + 0 = a)
+
+def AddNatSuccEqSucc 
+  {P : Sort u} (L : Logic P) (N : Type v) [LEq P N] [Nat P N] [Succ N] [Add N] := 
+  (a b : N) -> (L |- nat a) -> (L |- nat b) -> (L |- a + S b = S (a + b))
+
+-- Multiplication Axioms
+
+def MulNatZeroEqZero 
+  {P : Sort u} (L : Logic P) (N : Type v) [LEq P N] [Nat P N] [Zero N] [Mul N] :=
+  (a b : N) -> (L |- nat a) -> (L |- nat b) -> (L |- a * 0 = 0)
+
+def MulNatSuccEqAddMul 
+  {P : Sort u} (L : Logic P) (N : Type v) 
+  [LEq P N] [Nat P N] [Succ N] [Add N] [Mul N] := 
+  (a b : N) -> (L |- nat a) -> (L |- nat b) -> (L |- a + S b = a + S (a * b))
+
+end Gaea.Peano.Rules
