Gaea/Peano/Theorems.lean
@@ -1,0 +1,125 @@
+import Gaea.Logic
+import Gaea.Syntax
+import Gaea.Syntax.Notation
+import Gaea.Logic.Rules
+import Gaea.Peano.Rules
+
+universes u v w
+
+namespace Gaea.Peano
+
+open Gaea.Syntax
+open Gaea.Logic.Rules
+open Gaea.Peano.Rules
+
+-- General Theorems
+
+def natCases 
+{P : Sort u} {L : Logic P} {N : Type v} 
+[Nat P N] [Zero N] [Succ N]
+(natInduction : NatInduction L N)
+: (f : N -> P) -> 
+  (L |- f 0) -> ((n : N) -> (L |- nat n) -> (L |- f (S n))) -> 
+    ((n : N) -> (L |- nat n) -> (L |- f n))
+:= by
+  intro f f0 fS n nat_n
+  have ih : (n : N) -> (L |- nat n) -> (L |- f n) -> (L |- f (S n)) := 
+    fun n nat_n fn => fS n nat_n
+  exact natInduction f f0 ih n nat_n
+
+-- Addition Theorems
+
+theorem addZeroEqZero 
+{P : Sort u} {L : Logic P} {N : Type v} 
+[LEq P N] [Nat P N] [Zero N] [Add N] 
+(nat_0 : NatZero L N) 
+(An0_eq_n : AddNatZeroEqNat L N)
+: L |- 0 + 0 = (0 : N) 
+:= An0_eq_n 0 nat_0
+
+theorem natAddNatZero
+{P : Sort u} {L : Logic P} {N : Type v} 
+[LEq P N] [Nat P N] [Zero N] [Add N] 
+(natEq : NatEq L N) 
+(An0_eq_n : AddNatZeroEqNat L N)
+: (a : N) -> (L |- nat a) -> (L |- nat (a + 0))
+:= by
+  intro a nat_a
+  apply natEq _ a nat_a
+  exact An0_eq_n a nat_a
+
+theorem NatAddNat_induct
+{P : Sort u} {L : Logic P} {N : Type v} 
+[LForall P N] [LIf P] [LEq P N] [Nat P N] [Zero N] [Succ N] [Add N]
+(ifIntro : IfIntro L)
+(ifElim : IfElim L)
+(forallIntro : ForallIntro L N)
+(forallElim : ForallElim L N)
+(nat_S : NatSuccNat L N) 
+(natEq : NatEq L N) 
+(natInduction : NatInduction L N)
+(An0_eq_n : AddNatZeroEqNat L N)
+(AnS_eq_S : AddNatSuccEqSucc L N)
+: (b : N) -> (L |- nat b) -> (L |- forall (a : N) => nat a -> nat (a + b))
+:= by
+  intro b nat_b
+  apply natInduction 
+    (fun b => forall (a : N) => nat a -> nat (a + b))
+  -- Base
+  apply forallIntro; intro a
+  apply ifIntro; intro nat_a
+  exact natAddNatZero natEq An0_eq_n a nat_a
+  -- Induction
+  intro a nat_a p_ih
+  apply forallIntro; intro b
+  apply ifIntro; intro nat_b
+  have nat_Aba := ifElim _ _ (forallElim _ p_ih b) nat_b 
+  have abSa_eq_Saba := AnS_eq_S _ _ nat_b nat_a
+  have nat_SAba := nat_S _ nat_Aba
+  exact natEq _ _ nat_SAba abSa_eq_Saba
+  exact nat_b
+
+theorem NatAddNat'
+{P : Sort u} {L : Logic.{u,w} P} {N : Type v} 
+[LEq P N] [Nat P N] [Zero N] [Succ N] [Add N]
+(nat_S : NatSuccNat L N) 
+(natEq : NatEq L N) 
+(natInduction : NatInduction'.{u,v,(imax (v+1) w)} L N)
+(An0_eq_n : AddNatZeroEqNat L N)
+(AnS_eq_S : AddNatSuccEqSucc L N)
+: (a b : N) -> (L |- nat a) -> (L |- nat b) -> (L |- nat (a + b))
+:= by
+  intro m n nat_m nat_n
+  apply natInduction
+    (fun b => (a : N) -> (L |- nat a) -> (L |- nat (a + b)))
+  -- Base
+  intro a nat_a
+  exact natAddNatZero natEq An0_eq_n a nat_a
+  -- Induction
+  intro a nat_a ih b nat_b
+  have nat_Aba := ih b nat_b 
+  have abSa_eq_Saba := AnS_eq_S _ _ nat_b nat_a
+  have nat_SAba := nat_S _ nat_Aba
+  exact natEq _ _ nat_SAba abSa_eq_Saba
+  exact nat_n; exact nat_m
+
+theorem NatAddNat
+{P : Sort u} {L : Logic P} {N : Type v} 
+[LForall P N] [LIf P] [LEq P N] [Nat P N] [Zero N] [Succ N] [Add N]
+(ifIntro : IfIntro L)
+(ifElim : IfElim L)
+(forallIntro : ForallIntro L N)
+(forallElim : ForallElim L N)
+(nat_S : NatSuccNat L N) 
+(natEq : NatEq L N) 
+(natInduction : NatInduction L N)
+(An0_eq_n : AddNatZeroEqNat L N)
+(AnS_eq_S : AddNatSuccEqSucc L N)
+: (a b : N) -> (L |- nat a) -> (L |- nat b) -> (L |- nat (a + b))
+:= by
+  intro a b nat_a nat_b
+  have h :=  NatAddNat_induct ifIntro ifElim forallIntro forallElim  
+    nat_S natEq natInduction An0_eq_n AnS_eq_S b nat_b
+  exact ifElim _ _ (forallElim _ h a) nat_a
+
+end Gaea.Peano
