Gaea/Syntax.lean
@@ -1,0 +1,2 @@
+import Gaea.Syntax.Math
+import Gaea.Syntax.Logic
