Gaea/Syntax/Logic.lean
@@ -1,0 +1,58 @@
+universes u v
+
+namespace Gaea.Syntax 
+
+-- Constants
+
+class True (prop : Sort u) :=
+  (true : prop)
+
+export True (true)
+
+class False (prop : Sort u) :=
+  (false : prop)
+
+export False (false)
+
+-- Connectives
+
+class LIf (prop : Sort u) :=
+  (lif : prop -> prop -> prop)
+
+export LIf (lif)
+
+class LIff (prop : Sort u) :=
+  (liff : prop -> prop -> prop)
+
+export LIff (liff)
+
+class LAnd (prop : Sort u):=
+  (land : prop -> prop -> prop)
+
+export LAnd (land)
+
+class LOr (prop : Sort u) :=
+  (lor : prop -> prop -> prop)
+
+export LOr (lor)
+
+-- Equality
+
+class LEq (prop : Sort u) (form : Sort v) :=
+  (leq : form -> form -> prop)
+
+export LEq (leq)
+
+-- Quantifiers
+
+class LForall (prop : Sort u) (form : Sort v) :=
+  (lForall : (form -> prop) -> prop)
+
+export LForall (lForall)
+
+class LExists (prop : Sort u) (form : Sort v) :=
+  (lExists : (form -> prop) -> prop)
+
+export LExists (lExists)
+
+end Gaea.Syntax
