Gaea/Syntax/Notation.lean
@@ -1,0 +1,32 @@
+import Gaea.Syntax.Logic
+
+-- Connectives
+
+infixr:25 " -> " => Gaea.Syntax.LIf.lif
+infixr:25 " ⇒ " => Gaea.Syntax.LIf.lif
+
+infix:20 " <-> " => Gaea.Syntax.LIff.liff
+infix:20 " ⇔ "  => Gaea.Syntax.LIff.liff
+
+infixr:35 " /\\ " => Gaea.Syntax.LAnd.land
+infixr:35 " ∧ "   => Gaea.Syntax.LAnd.lor
+infixr:30 " \\/ " => Gaea.Syntax.LOr.lor
+infixr:30 " ∨ "   => Gaea.Syntax.LOr.lor
+
+-- Equality
+
+infix:50 " = "  => Gaea.Syntax.LEq.leq
+
+-- Quantifiers
+
+open Lean
+
+macro "∀" xs:explicitBinders " => " b:term : term => 
+  expandExplicitBinders `Gaea.Syntax.LForall.lForall xs b
+macro "forall" xs:explicitBinders " => " b:term : term => 
+  expandExplicitBinders `Gaea.Syntax.LForall.lForall xs b
+
+macro "∃" xs:explicitBinders " => " b:term : term => 
+  expandExplicitBinders `Gaea.Syntax.LExists.lExists xs b
+macro "exists" xs:explicitBinders " => " b:term : term => 
+  expandExplicitBinders `Gaea.Syntax.LExists.lExists xs b
